trunk/color/NonTermin/ALoop.v
@@ -14,245 +14,243 @@ Require Import LogicUtil ATrs ListUtil.
 
 Section S.
 
-Variable Sig : Signature.
+  Variable Sig : Signature.
 
-Notation term := (term Sig). Notation context := (context Sig).
-Notation substitution := (substitution Sig).
-Notation rule := (rule Sig). Notation rules := (list rule).
+  Notation term := (term Sig). Notation beq_rule := (@beq_rule Sig).
 
-Notation beq_rule := (@beq_rule Sig).
-
-Variable R : rules.
+  Variable R : rules Sig.
 
 (***********************************************************************)
 (** predicates saying that [t::us] is in a sequence of rewriting steps *)
 
-Fixpoint FS t us :=
-  match us with
-    | nil => True
-    | u :: us' => red R t u /\ FS u us'
-  end.
+  Fixpoint FS t us :=
+    match us with
+      | nil => True
+      | u :: us' => red R t u /\ FS u us'
+    end.
 
-Definition terms_of_reduc : forall t, {us| FS t us} -> list term.
+  Definition terms_of_reduc : forall t, {us| FS t us} -> list term.
 
-Proof.
-intros t x. destruct x. exact x.
-Defined.
+  Proof.
+    intros t x. destruct x. exact x.
+  Defined.
 
-Implicit Arguments terms_of_reduc [t].
+  Implicit Arguments terms_of_reduc [t].
 
-Definition proof_of_reduc :
-  forall t, forall x : {us| FS t us}, FS t (terms_of_reduc x).
+  Definition proof_of_reduc :
+    forall t, forall x : {us| FS t us}, FS t (terms_of_reduc x).
 
-Proof.
-intros t x. destruct x. exact f.
-Defined.
+  Proof.
+    intros t x. destruct x. exact f.
+  Defined.
 
-Require Import RelUtil.
+  Require Import RelUtil.
 
-Lemma FS_rtc : forall us t, FS t us -> red R # t (last us t).
+  Lemma FS_rtc : forall us t, FS t us -> red R # t (last us t).
 
-Proof.
-induction us. simpl. intros. apply rt_refl. simpl FS. intuition.
-apply rt_trans with a. apply rt_step. hyp. simpl. destruct us. apply rt_refl.
-rewrite last_default with (d2:=a). apply IHus. hyp. discr.
-Qed.
+  Proof.
+    induction us. simpl. intros. apply rt_refl. simpl FS. intuition.
+    apply rt_trans with a. apply rt_step. hyp. simpl. destruct us.
+    apply rt_refl. rewrite last_default with (d2:=a). apply IHus. hyp. discr.
+  Qed.
 
 (***********************************************************************)
 (** data necessary for a sequence of rewrite steps *)
 
-Require Import AMatching ListDec APosition.
+  Require Import AMatching ListDec APosition.
 
-Definition data := (position * rule)%type.
+  Definition data := (position * rule Sig)%type.
 
-Definition rewrite (t : term) (d : data) : option term :=
-  let (p,a) := d in let (l,r) := a in
-    if mem beq_rule (mkRule l r) R then
-      match subterm_pos t p with
-        | None => None
-        | Some u =>
-          match matches l u with
-            | None => None
-            | Some s => replace_pos t p (sub s r)
-          end
-      end
-      else None.
+  Definition rewrite (t : term) (d : data) : option term :=
+    let (p,a) := d in let (l,r) := a in
+      if mem beq_rule (mkRule l r) R then
+        match subterm_pos t p with
+          | None => None
+          | Some u =>
+            match matches l u with
+              | None => None
+              | Some s => replace_pos t p (sub s r)
+            end
+        end
+        else None.
 
-Lemma rewrite_correct : forall t d u, rewrite t d = Some u -> red R t u.
+  Lemma rewrite_correct : forall t d u, rewrite t d = Some u -> red R t u.
 
-Proof.
-intros t [p [l r]] u. unfold rewrite.
-case_eq (mem beq_rule (mkRule l r) R). 2: discr.
-gen H0. case_eq (subterm_pos t p). 2: discr.
-gen H1. case_eq (matches l t0). rename t1 into s. 2: discr.
-rewrite red_pos_ok. exists p. exists l. exists r. exists s. intuition.
-rewrite mem_ok in H. hyp. apply beq_rule_ok.
-ded (matches_correct H1). rewrite H3. hyp.
-Qed.
+  Proof.
+    intros t [p [l r]] u. unfold rewrite.
+    case_eq (mem beq_rule (mkRule l r) R). 2: discr.
+    gen H0. case_eq (subterm_pos t p). 2: discr.
+    gen H1. case_eq (matches l t0). rename t1 into s. 2: discr.
+    rewrite red_pos_ok. exists p. exists l. exists r. exists s. intuition.
+    rewrite mem_ok in H. hyp. apply beq_rule_ok.
+    ded (matches_correct H1). rewrite H3. hyp.
+  Qed.
 
-Implicit Arguments rewrite_correct [t d u].
+  Implicit Arguments rewrite_correct [t d u].
 
-Fixpoint rewrites t (ds : list data) : option (list term) :=
-  match ds with
-    | nil => Some nil
-    | d :: ds' =>
-      match rewrite t d with
-        | None => None
-        | Some u =>
-          match rewrites u ds' with
-            | None => None
-            | Some us => Some (u::us)
-          end
-      end
-  end.
+  Fixpoint rewrites t (ds : list data) : option (list term) :=
+    match ds with
+      | nil => Some nil
+      | d :: ds' =>
+        match rewrite t d with
+          | None => None
+          | Some u =>
+            match rewrites u ds' with
+              | None => None
+              | Some us => Some (u::us)
+            end
+        end
+    end.
 
-Lemma rewrites_correct : forall ds t us, rewrites t ds = Some us -> FS t us.
+  Lemma rewrites_correct : forall ds t us, rewrites t ds = Some us -> FS t us.
 
-Proof.
-induction ds; simpl; intros. inversion H. exact I.
-gen H. case_eq (rewrite t a). 2: discr.
-gen H0. case_eq (rewrites t0 ds). 2: discr.
-inversion H1. simpl. ded (rewrite_correct H). intuition.
-Qed.
+  Proof.
+    induction ds; simpl; intros. inversion H. exact I.
+    gen H. case_eq (rewrite t a). 2: discr.
+    gen H0. case_eq (rewrites t0 ds). 2: discr.
+    inversion H1. simpl. ded (rewrite_correct H). intuition.
+  Qed.
 
-Implicit Arguments rewrites_correct [ds t us].
+  Implicit Arguments rewrites_correct [ds t us].
 
-Require Import NatUtil.
+  Require Import NatUtil.
 
-Notation default := (Var 0).
+  Notation default := (Var 0).
 
-Lemma FS_red : forall ts t, FS t ts -> forall i, i < length ts ->
-  red R (nth i (t::ts) default) (nth (S i) (t::ts) default).
+  Lemma FS_red : forall ts t, FS t ts -> forall i, i < length ts ->
+    red R (nth i (t::ts) default) (nth (S i) (t::ts) default).
 
-Proof.
-induction ts; simpl; intros. absurd_arith. destruct H. destruct i. hyp.
-ded (IHts _ H1 i (lt_S_n H0)). hyp.
-Qed.
+  Proof.
+    induction ts; simpl; intros. absurd_arith. destruct H. destruct i. hyp.
+    ded (IHts _ H1 i (lt_S_n H0)). hyp.
+  Qed.
 
 (***********************************************************************)
 (** assumptions for non-termination *)
 
-Section loop.
+  Section loop.
 
-Variables (t : term) (ds : list data)
-  (us : list term) (h1 : rewrites t ds = Some us).
+    Variables (t : term) (ds : list data)
+      (us : list term) (h1 : rewrites t ds = Some us).
 
-Definition k := length us.
+    Definition k := length us.
 
-Definition nth i := nth i us default.
+    Definition nth i := nth i us default.
 
-Definition last_term := nth (k-1).
+    Definition last_term := nth (k-1).
 
-Variables (h0 : k > 0).
+    Variable h0 : k > 0.
 
-Lemma FS_red' : forall i, i < k - 1 -> red R (nth i) (nth (S i)).
+    Lemma FS_red' : forall i, i < k - 1 -> red R (nth i) (nth (S i)).
 
-Proof.
-intros. unfold nth.
-change (red R (List.nth (S i) (t :: us) default)
-  (List.nth (S (S i)) (t :: us) default)).
-apply FS_red. eapply rewrites_correct. apply h1. unfold k in *. omega.
-Qed.
+    Proof.
+      intros. unfold nth.
+      change (red R (List.nth (S i) (t :: us) default)
+        (List.nth (S (S i)) (t :: us) default)).
+      apply FS_red. eapply rewrites_correct. apply h1. unfold k in *. omega.
+    Qed.
 
-Variables (p : position) (u : term) (h2 : subterm_pos last_term p = Some u)
-  (s : substitution) (h3 : matches t u = Some s).
+    Variables (p : position) (u : term) (h2 : subterm_pos last_term p = Some u)
+      (s : substitution Sig) (h3 : matches t u = Some s).
 
 (***********************************************************************)
 (** proof of non-termination *)
 
-Definition c : context.
+    Definition c : context Sig.
 
-Proof.
-destruct (subterm_pos_elim h2). exact x.
-Defined.
+    Proof.
+      destruct (subterm_pos_elim h2). exact x.
+    Defined.
 
-Definition g t := fill c (sub s t).
+    Definition g t := fill c (sub s t).
 
-Lemma last_term_g : last_term = g t.
+    Lemma last_term_g : last_term = g t.
 
-Proof.
-unfold g, c. destruct (subterm_pos_elim h2). destruct a.
-rewrite H0. ded (matches_correct h3). subst u. refl.
-Qed.
+    Proof.
+      unfold g, c. destruct (subterm_pos_elim h2). destruct a.
+      rewrite H0. ded (matches_correct h3). subst u. refl.
+    Qed.
 
-Lemma red_g : forall a b, red R a b -> red R (g a) (g b).
+    Lemma red_g : forall a b, red R a b -> red R (g a) (g b).
 
-Proof.
-intros. apply red_fill. apply red_sub. hyp.
-Qed.
+    Proof.
+      intros. apply red_fill. apply red_sub. hyp.
+    Qed.
 
-Require Import Euclid.
+    Require Import Euclid.
 
-Definition seq : nat -> term.
+    Definition seq : nat -> term.
 
-Proof.
-intro n. destruct (eucl_dev k h0 n). exact (iter (nth r) g q).
-Defined.
+    Proof.
+      intro n. destruct (eucl_dev k h0 n). exact (iter (nth r) g q).
+    Defined.
 
-Require Import RelUtil Wf_nat.
+    Require Import RelUtil Wf_nat.
 
-Lemma IS_seq : IS (red R) seq.
+    Lemma IS_seq : IS (red R) seq.
 
-Proof.
-intro n; pattern n; apply lt_wf_ind; clear n; intros. unfold seq at -2 .
-destruct (eucl_dev k h0 n); simpl. destruct (le_gt_dec (k-1) r).
-(* r = k-1 *)
-assert (r = k-1). omega. assert (S n = (S q)*k + 0). rewrite mult_succ_l.
-omega. rewrite H1. unfold seq. destruct (eucl_dev k h0 (S q * k + 0)).
-destruct (eucl_div_unique h0 g1 e0). rewrite <- H3. rewrite <- H2. simpl.
-rewrite <- iter_com. apply red_iter. apply red_g.
-rewrite H0. fold last_term. rewrite last_term_g.
-apply red_g. unfold nth.
-change (red R (List.nth 0 (t :: us) default) (List.nth 1 (t :: us) default)).
-apply FS_red. apply (rewrites_correct h1). hyp.
-(* r < k-1 *)
-assert (S n = q*k + S r). omega. rewrite H0. unfold seq.
-destruct (eucl_dev k h0 (q * k + S r)). assert (k>S r). omega.
-destruct (eucl_div_unique H1 g2 e0). rewrite <- H3. rewrite <- H2.
-apply red_iter. apply red_g. apply FS_red'. omega.
-Qed.
+    Proof.
+      intro n; pattern n; apply lt_wf_ind; clear n; intros. unfold seq at -2 .
+      destruct (eucl_dev k h0 n); simpl. destruct (le_gt_dec (k-1) r).
+      (* r = k-1 *)
+      assert (r = k-1). omega. assert (S n = (S q)*k + 0). rewrite mult_succ_l.
+      omega. rewrite H1. unfold seq. destruct (eucl_dev k h0 (S q * k + 0)).
+      destruct (eucl_div_unique h0 g1 e0). rewrite <- H3. rewrite <- H2. simpl.
+      rewrite <- iter_com. apply red_iter. apply red_g.
+      rewrite H0. fold last_term. rewrite last_term_g.
+      apply red_g. unfold nth.
+      change (red R (List.nth 0 (t :: us) default)
+        (List.nth 1 (t :: us) default)).
+      apply FS_red. apply (rewrites_correct h1). hyp.
+      (* r < k-1 *)
+      assert (S n = q*k + S r). omega. rewrite H0. unfold seq.
+      destruct (eucl_dev k h0 (q * k + S r)). assert (k>S r). omega.
+      destruct (eucl_div_unique H1 g2 e0). rewrite <- H3. rewrite <- H2.
+      apply red_iter. apply red_g. apply FS_red'. omega.
+    Qed.
 
-Lemma loop : EIS (red R).
+    Lemma loop : EIS (red R).
 
-Proof.
-exists seq. apply IS_seq.
-Qed.
+    Proof.
+      exists seq. apply IS_seq.
+    Qed.
 
-End loop.
+  End loop.
 
 (***********************************************************************)
 (** boolean function testing non-termination *)
 
-Definition is_loop t ds p :=
-  match rewrites t ds with
-    | None => false
-    | Some us =>
-      match us with
-        | nil => false
-        | _ =>
-          let u := last us default in
-            match subterm_pos u p with
-              | None => false
-              | Some v =>
-                match matches t v with
-                  | None => false
-                  | Some _ => true
-                end
-            end
-      end
-  end.
+  Definition is_loop t ds p :=
+    match rewrites t ds with
+      | None => false
+      | Some us =>
+        match us with
+          | nil => false
+          | _ =>
+            let u := last us default in
+              match subterm_pos u p with
+                | None => false
+                | Some v =>
+                  match matches t v with
+                    | None => false
+                    | Some _ => true
+                  end
+              end
+        end
+    end.
 
-Lemma is_loop_correct : forall t ds p, is_loop t ds p = true -> EIS (red R).
+  Lemma is_loop_correct : forall t ds p, is_loop t ds p = true -> EIS (red R).
 
-Proof.
-intros t ds p. unfold is_loop. coq_case_eq (rewrites t ds). 2: discr.
-destruct l. discr. set (us := t0::l). set (u := last us default).
-coq_case_eq (subterm_pos u p). 2: discr. intro v. case_eq (matches t v).
-2: discr. assert (h0 : k us > 0). unfold k, us. simpl. omega.
-assert (h : u = last_term us). unfold last_term, k, nth. rewrite <- last_nth.
-refl. rewrite h in H0. exists (seq us h0 p H0 t1). eapply IS_seq. apply H1.
-hyp.
-Qed.
+  Proof.
+    intros t ds p. unfold is_loop. coq_case_eq (rewrites t ds). 2: discr.
+    destruct l. discr. set (us := t0::l). set (u := last us default).
+    coq_case_eq (subterm_pos u p). 2: discr. intro v. case_eq (matches t v).
+    2: discr. assert (h0 : k us > 0). unfold k, us. simpl. omega.
+    assert (h : u = last_term us). unfold last_term, k, nth.
+    rewrite <- last_nth.
+    refl. rewrite h in H0. exists (seq us h0 p H0 t1). eapply IS_seq. apply H1.
+    hyp.
+  Qed.
 
 End S.
 
